minimal custom impl of gcongr working

Lean4Axiomatic/Tactic/Sandbox.lean
@@ -3,7 +3,7 @@ import Mathlib.Tactic.GCongr
 
 namespace Lean4Axiomatic.Tactic
 
-open Lean (Expr MVarId Syntax getExprMVarAssignment? withRef)
+open Lean (Expr MVarId Name Syntax getExprMVarAssignment? withRef)
 open Lean.Elab.Tactic (
   Tactic TacticM getMainGoal getMainTarget replaceMainGoal withMainContext
   withRWRulesSeq
@@ -11,7 +11,7 @@ open Lean.Elab.Tactic (
 open Lean.Elab.Term (elabTerm)
 open Lean.Meta (
   MetaM isDefEq isProof mkConstWithFreshMVarLevels
-  mkFreshExprSyntheticOpaqueMVar saveState withReducible
+  mkFreshExprSyntheticOpaqueMVar saveState whnf withReducible
   withReducibleAndInstances
 )
 open Lean.MonadEnv (getEnv)
@@ -20,6 +20,55 @@ open Lean.Parser.Tactic (rwRuleSeq)
 open Mathlib.Tactic.GCongr (
   gcongrExt gcongrForwardDischarger getCongrAppFnArgs getRel
 )
+
+def getRel : Expr → Option (Name × Expr × Expr)
+| .app (.app rel lhs) rhs => rel.getAppFn.constName?.map (·, lhs, rhs)
+| _ => none
+
+partial def scongr? (goal : MVarId) : TacticM Unit := goal.withContext do
+  -- Try to solve goal right away
+  try
+    gcongrForwardDischarger goal
+    return ()
+  catch _ =>
+    pure ()
+
+  -- Validate goal is in the right shape for this tactic
+  let rel ← goal.getType -- Not reducing to whnf until needed
+  let some (relName, lhs, rhs) := getRel rel | throwError "scongr?: not rel"
+  let some (lhsHead, lhsArgs) := getCongrAppFnArgs lhs | throwError "lhs bad"
+  let some (rhsHead, rhsArgs) := getCongrAppFnArgs rhs | throwError "rhs bad"
+  unless lhsHead == rhsHead && lhsArgs.size == rhsArgs.size do
+    throwError "mismatched lhs & rhs"
+  let varyingArgs ← (lhsArgs.zip rhsArgs).mapM λ (lhsArg, rhsArg) => do
+    let argsEq ← isDefEq lhsArg rhsArg
+    -- Considering proofs equal may need to be updated
+    let isSame := argsEq || (← isProof lhsArg) && (← isProof rhsArg)
+    return !isSame
+  if varyingArgs.all not then throwError "args are all same; use rfl instead?"
+
+  -- Apply the first lemma that matches
+  let key := { relName, head := lhsHead, varyingArgs }
+  let matchingLemmas := (gcongrExt.getState (← getEnv)).getD key #[]
+  let s ← saveState
+  let lemAndNewGoalsOpt ← matchingLemmas.findSomeM? λ lem =>
+    try
+      let gs ← goal.apply (.const lem.declName [])
+      dbg_trace "scongr?: applied {lem.declName} successfully"
+      return some (lem, gs)
+    catch _ =>
+      s.restore
+      return none
+  let some (lem, _newGoals) := lemAndNewGoalsOpt | return ()
+
+  -- Recursively apply this tactic to main subgoals
+  let some e ← getExprMVarAssignment? goal | panic! "goal unassigned?"
+  let args := e.getAppArgs
+  for (i, _, _) in lem.mainSubgoals do
+    let some (.mvar mvarId) := args[i]? | panic! "hyp not an mvar?"
+    scongr? mvarId
+
+elab "scongr?" : tactic => do scongr? (← getMainGoal)
 
 partial def scongr
     (goal : MVarId)
